Working on IP, in progress

proofs/FEC/IP.v
@@ -1,5 +1,8 @@
 Require Import Endian.
 Require Import VST.floyd.functional_base.
+From RecordUpdate Require Import RecordSet. (*for updating records easily*)
+Import RecordSetNotations.
+Set Bullet Behavior "Strict Subproofs".
 
 (** IP and UDP Packets *)
 
@@ -12,6 +15,9 @@ Record ip_fields :=
   mk_ip { ip_hl : nibble; ip_v : nibble; ip_tos : byte; ip_len : short; ip_id : short; ip_off : short;
     ip_ttl: byte; ip_p: byte; ip_sum : short; ip_src : int; ip_dst: int; ip_options: list byte}.
 
+#[export]Instance eta_ip_fields: Settable _ := 
+  settable! mk_ip <ip_hl; ip_v; ip_tos; ip_len; ip_id; ip_off; ip_ttl; ip_p; ip_sum; ip_src; ip_dst; ip_options>.
+
 Definition ip_list (f: ip_fields) :=
   let e:= BigEndian in
   [NibbleMem (ip_hl f) (ip_v f); ByteMem (ip_tos f); ShortMem (ip_len f) e; ShortMem (ip_id f) e;
@@ -22,34 +28,78 @@ Definition ip_bytes (f: ip_fields) :=
   MemBytes_to_byte_list (ip_list f) ++ (ip_options f).
 
 (*TODO: do we need any other validity conditions?*)
-Definition valid_ip_bytes (f: ip_fields) (contents: list byte) : Prop :=
-  Nibble.unsigned (ip_hl f) * 4 = Zlength (ip_bytes f) /\
-  Short.unsigned (ip_len f) = Zlength (ip_bytes f ++ contents).
+Definition valid_ip_bytes (f: ip_fields) (contents: list byte) : bool :=
+  Z.eq_dec (Nibble.unsigned (ip_hl f) * 4) (Zlength (ip_bytes f)) &&
+  Z.eq_dec (Short.unsigned (ip_len f)) (Zlength (ip_bytes f ++ contents)).
 
-(* Now we need to go to the other way: header bytes -> ip_fields*)
-(*TODO:*)
-Definition packet_to_ip_fields (packet: list byte) : option ip_fields :=
-  match packet with
+(*Fixed parts of IP packet take up 20 bytes*) 
+
+(*Suppose we are given the header along with the packet contents. We want to reconstruct the fields and
+  define a validity predicate*)
+
+(*Get header fields from a list of bytes representing the header*)
+Definition bytes_to_header_fields (header: list byte) : option (ip_fields) :=
+  match header with
   | ip_hlv :: ip_tos :: ip_len1 :: ip_len2 :: ip_id1 :: ip_id2 :: ip_off1 :: ip_off2 ::
     ip_tll :: ip_p :: ip_sum1 :: ip_sum2 :: ip_src1 :: ip_src2 :: ip_src3 :: ip_src4 ::
-    ip_dst1 :: ip_dst2 :: ip_dst3 :: id_dst4 :: rest =>
-      mk_ip 
-
-
-
-  | _ => None
-    
+    ip_dst1 :: ip_dst2 :: ip_dst3 :: ip_dst4 :: rest =>
+      let E := BigEndian in
+      let (ip_hl, ip_v) := byte_to_nibbles ip_hlv in
+        Some (mk_ip ip_hl ip_v ip_tos (bytes_to_short E ip_len1 ip_len2) (bytes_to_short E ip_id1 ip_id2)
+        (bytes_to_short E ip_off1 ip_off2) ip_tll ip_p (bytes_to_short E ip_sum1 ip_sum2)
+        (bytes_to_int E ip_src1 ip_src2 ip_src3 ip_src4)
+        (bytes_to_int E ip_dst1 ip_dst2 ip_dst3 ip_dst4) rest)
   | _ => None
   end.
-  | nil => None
-  | 
 
+Definition packet_to_ip_fields (packet: list byte) : option (ip_fields * list byte) :=
+  match (bytes_to_header_fields packet) with
+  | Some i => 
+    let realOptions := sublist 20 (4 * Nibble.unsigned (ip_hl i)) packet in
+    let contents := sublist (4 * Nibble.unsigned (ip_hl i)) (Short.unsigned (ip_len i)) packet in
+    Some (i <| ip_options := realOptions |>, contents)
+  | None => None
+  end.
 
+(*Given the header and contents, we want to define a validity predicate*)
+Definition valid_packet (header: list byte) (contents: list byte) : bool :=
+  match (bytes_to_header_fields header) with
+  | Some i => Z.eq_dec (4 * Nibble.unsigned (ip_hl i)) (Zlength header) &&  
+              Z.eq_dec (Short.unsigned (ip_len i)) (Zlength (header ++ contents))
+  | None => false
+  end.
 
+(*Get header and contents from a packet*)
+Definition recover_packet (pack: list byte) : (list byte * list byte) :=
+  match (packet_to_ip_fields pack) with
+  | None => (nil, nil)
+  | Some (i, con) => (ip_bytes i, con)
+  end.
 
-Definition valid_ip_bytes (f: ip_fields) (options: list byte) (contents: list byte) : Prop :=
-  Nibble.unsigned (ip_hl f) * 4 = Zlength (ip_bytes f options) /\
-  Short.unsigned (ip_len f) = Zlength (ip_bytes f options ++ contents).
+Ltac solve_con:=
+  solve[ let H := fresh in
+  intros H; inversion H].
+
+(*The main theorem we need*)
+
+(*KEY! what we want: bytes_to_header_fields header = Some ip <-> ip_bytes ip = header
+(maybe, not as sure although this may help me prove the next lemma)
+
+  WANT: bytes_to_header_fields header = Some ip ->
+  bytes_to_header_fields header ++ l = Some ip' ->
+  (forall fields other than contents, ip.f = ip'.f)
+
+then we reason as follows (to show that recover_packet gives (header, contents)
+  want to show that ip_bytes ip' = header - USE ABOVE LEMMA and equality from above
+  and then contents, reason about sublist and length
+
+THESE TWO LEMMAS ARE WHAT WE NEED
+
+Lemma recover_packet_correct: forall (header contents : list byte) (extra: list byte),
+  valid_packet header contents = true ->
+  recover_packet (header ++ contents ++ extra) = (header, contents).
+Proof.
+*)
 
 (** UDP *)
 
